Core/Metatheory/Progress.lean
@@ -13,7 +13,15 @@ theorem spctor_inversion :
   G&Δ,Γ ⊢ Term.spctor v s tys ts : T ->
   T.spine.isSome
 := by
+  intro j1 j2
+  cases j2; case _ j2 j3 j4 j5 j6 j7 j8 =>
+  cases v <;> simp at j1; case _ c =>
+  replace j4 := j4 c rfl; subst j8
   sorry
+
+theorem Query.subst_invariant {T : Vec Ty n} (σ : Subst Ty)
+  : Query G q (Vec.map (·[σ]) T) -> Query G q T
+:= sorry
 
 theorem split_all_or_left : ∀ {n} {A B : Fin n -> Prop}, (∀ i, A i ∨ B i) -> (∀ i, A i) ∨ (∃ i, B i)
 | 0, _, _, _ => Or.inl (Fin.elim0 ·)
@@ -35,97 +43,112 @@ def Constructor.query : Vec Constructor n -> Vec String n
 theorem Constructor.query_nil : {c : Vec Constructor 0} -> query c = .nil -> c = .nil
 | .nil, _ => rfl
 
--- theorem Constructor.query_cons {qs : Vec _ _} :
---   {c : Vec Constructor (n + 1)} ->
---   query c = q::qs ->
---   ∃ As ts, ∃ (cs : Vec _ _), c = (q,As,ts)::cs ∧ query cs = qs
--- | .cons (s, As, ts) tl, e =>
---   have lem : s = q ∧ query tl = qs := by simp at e; exact e
---   ⟨As, ts, tl, by rw [lem.1]; rfl, lem.2⟩
+theorem Constructor.query_cons {qs : Vec _ _} :
+  {c : Vec Constructor (n + 1)} ->
+  query c = q::qs ->
+  ∃ na nt As ts, ∃ (cs : Vec _ _), c = ⟨q,na,As,nt,ts⟩::cs ∧ query cs = qs
+| .cons ⟨s, na, As, nt, ts⟩ tl, e =>
+  have lem : s = q ∧ query tl = qs := by simp at e; exact e
+  ⟨na, nt, As, ts, tl, by rw [lem.1], lem.2⟩
 
--- theorem progress_match_ctors_head {ctors : Vec _ n} :
---   G&Δ,Γ ⊢ s : S ->
---   Ty.datatype? G S ->
---   Value G s ->
---   Term.IsData .cdata ss ctors ->
---   Query G (Constructor.query ctors) SS ->
---   ∃ ctors, Term.IsData SpCtorVariant.cdata (s :: ss) ctors ∧ Query G (Constructor.query ctors) (S :: SS)
--- | .spctor (v := .cdata) (ctor := c) (As := As) (ts := ts) j1 j2 j3 j4 j5 j6, h2, .spctor h, h4, h5 =>
---   let ts' := Vec.to_list ts.to
---   let lem1 := @Term.IsData.cons .cdata ts' n ss ctors c As _ ts rfl h4
---   let lem2 : Ty.ctor? G c S := by {
---     simp [Ty.datatype?, Ty.HeadVariable] at h2
---     simp [Ty.ctor?]
---     sorry -- obvious, should rework global stuff so that we can just grind this
---   }
---   let lem3 := @Query.cons G _ (Constructor.query ctors) SS c S lem2 h5
---   ⟨⟨c, As, ts'⟩::ctors, lem1, lem3⟩
--- | .spctor (v := .odata) (ctor := c) (As := As) (ts := ts) j1 j2 j3 j4 j5 j6, h2, .spctor h, h4, h5 =>
---   sorry -- impossible by j6 and h2
--- | .refl j, h2, .refl, h4, h5 => by simp [Ty.datatype?, Ty.HeadVariable, Ty.spine] at h2
--- | .lam j1 j2, h2, .lam, h4, h5 => by simp [Ty.datatype?, Ty.HeadVariable, Ty.spine] at h2
--- | .lamt j1 j2, h2, .lamt, h4, h5 => by simp [Ty.datatype?, Ty.HeadVariable, Ty.spine] at h2
+theorem progress_match_ctors_head {ctors : Vec _ n} :
+  G&Δ,Γ ⊢ s : S ->
+  Ty.data? cv G S ->
+  Value G s ->
+  Term.IsData cv ss ctors ->
+  Query G (Constructor.query ctors) SS ->
+  ∃ ctors, Term.IsData cv (s :: ss) ctors ∧ Query G (Constructor.query ctors) (S :: SS)
+| .spctor (v := .data .cls) (As := As) (ts := ts) j1 j2 j3 j4 j5 j6 j7, h2, .spctor h, h4, h5 =>
+  sorry
+  -- let ts' := Vec.to_list ts.to
+  -- let lem1 := @Term.IsData.cons .cdata ts' n ss ctors c As _ ts rfl h4
+  -- let lem2 : Ty.ctor? G c S := by {
+  --   simp [Ty.datatype?, Ty.HeadVariable] at h2
+  --   simp [Ty.ctor?]
+  --   sorry -- obvious, should rework global stuff so that we can just grind this
+  -- }
+  -- let lem3 := @Query.cons G _ (Constructor.query ctors) SS c S lem2 h5
+  -- ⟨⟨c, As, ts'⟩::ctors, lem1, lem3⟩
+| .spctor (v := .data .opn) (As := As) (ts := ts) j1 j2 j3 j4 j5 j6 j7, h2, .spctor h, h4, h5 =>
+  sorry
+| .refl j, h2, .refl, h4, h5 => by simp [Ty.data?, Ty.HeadVariable, Ty.spine] at h2
+| .lam j1 j2, h2, .lam, h4, h5 => by simp [Ty.data?, Ty.HeadVariable, Ty.spine] at h2
+| .lamt j1 j2, h2, .lamt, h4, h5 => by simp [Ty.data?, Ty.HeadVariable, Ty.spine] at h2
 
--- theorem progress_match_ctors :
---   {m : Nat} ->
---   {S ss : Vec _ m} ->
---   (∀ (i : Fin m), G&Δ,Γ ⊢ ss[i] : S[i]) ->
---   (∀ (i : Fin m), Ty.datatype? G S[i]) ->
---   (∀ (i : Fin m), Value G ss[i]) ->
---   ∃ ctors, Term.IsData .cdata ss ctors ∧ Query G (Constructor.query ctors) S
--- | 0, .nil, .nil, h1, h2, h3 => ⟨.nil, Term.IsData.nil, Query.nil⟩
--- | m + 1, .cons Shd S, .cons shd s, h1, h2, h3 =>
---   let h1' : ∀ (i : Fin m), G&Δ,Γ ⊢ s[i] : S[i] := λ i => h1 i.succ
---   let h2' : ∀ (i : Fin m), Ty.datatype? G S[i] := λ i => h2 i.succ
---   let h3' : ∀ (i : Fin m), Value G s[i] := λ i => h3 i.succ
---   let ⟨ctors, q1, q2⟩ := progress_match_ctors h1' h2' h3'
---   progress_match_ctors_head (h1 0) (h2 0) (h3 0) q1 q2
+theorem progress_match_ctors :
+  {m : Nat} ->
+  {S ss : Vec _ m} ->
+  (∀ (i : Fin m), G&Δ,Γ ⊢ ss[i] : S[i]) ->
+  (∀ (i : Fin m), Ty.data? c G S[i]) ->
+  (∀ (i : Fin m), Value G ss[i]) ->
+  ∃ ctors, Term.IsData c ss ctors ∧ Query G (Constructor.query ctors) S
+| 0, .nil, .nil, h1, h2, h3 => ⟨.nil, Term.IsData.nil, Query.nil⟩
+| m + 1, .cons Shd S, .cons shd s, h1, h2, h3 =>
+  let h1' : ∀ (i : Fin m), G&Δ,Γ ⊢ s[i] : S[i] := λ i => h1 i.succ
+  let h2' : ∀ (i : Fin m), Ty.data? c G S[i] := λ i => h2 i.succ
+  let h3' : ∀ (i : Fin m), Value G s[i] := λ i => h3 i.succ
+  let ⟨ctors, q1, q2⟩ := progress_match_ctors h1' h2' h3'
+  progress_match_ctors_head (h1 0) (h2 0) (h3 0) q1 q2
 
--- theorem query_match_implies_pattern_match :
---   Constructor.query c = q ->
---   Query.Match q p ->
---   Pattern.Match c p
--- | e, .nil => Pattern.Match.nil |> cast (by rw [Constructor.query_nil e])
--- | e, .cons (ts := Bs) (n := n) tl =>
---   let ⟨As, ts, cs, h1, h2⟩ := Constructor.query_cons e
---   let tl' := query_match_implies_pattern_match h2 tl
---   by rw [h1]; apply Pattern.Match.cons tl'
+theorem query_match_implies_pattern_match :
+  {n : Nat} ->
+  {c : Vec Constructor n} ->
+  {q : Vec String n} ->
+  {p : Pattern n} ->
+  Constructor.query c = q ->
+  Query.Match q p ->
+  Pattern.Match c p
+| 0, .nil, .nil, .nil, e, .nil => Pattern.Match.nil |> cast (by rw [Constructor.query_nil e])
+| n + 1, .cons c cs, .cons q qs, .cons ⟨q', na, As, nb⟩ ps, e, .cons tl e2 =>
+  let ⟨na, nt, As, ts, cs, h1, h2⟩ := Constructor.query_cons e
+  let tl' := query_match_implies_pattern_match h2 tl
+  sorry
+  -- by rw [h1]; apply Pattern.Match.cons tl';
 
-theorem progress :
+theorem progress (oe : OpenExhaustive G) :
   G&Δ,Γ ⊢ t : T ->
   Γ = [] ->
   Value G t ∨ ∃ t', G ⊢ t ~> t'
-| .defn j1 j2, e => sorry
+| .defn j1 j2, e => Or.inr ⟨_, .defn j1⟩
 | .spctor (v := .data .cls) j1 j2 j3 j4 j5 j6 j7, e => Or.inl $ Value.spctor (by simp)
 | .spctor (v := .data .opn) j1 j2 j3 j4 j5 j6 j7, e => Or.inl $ Value.spctor (by simp)
-| .spctor (v := .openm) (ts := ts) j1 j2 j3 j4 j5 j6 j7, e =>
-  let j4' := λ i => progress (j4 i) e
+| @Typing.spctor G m n x Ks Ts R Δ τ Γ .openm R' As ts j1 j2 j3 j4 j5 j6 j7, e =>
+  let j4' := λ i => progress oe (j4 i) e
   match split_all_or_left j4' with
   | Or.inl vs =>
-    sorry
+    let Ts' : Vec Ty n := Vec.map (·[τ]) Ts
+    let j1' : ∀ (i : Fin n), G&Δ,Γ ⊢ ts.to[i] : Ts'[i] := sorry
+    let j2' : ∀ (i : Fin n), Ty.data? .opn G Ts'[i] := sorry
+    let vs' : ∀ (i : Fin n), Value G ts.to[i] := vs |> cast (by simp)
+    let ⟨ctors, h1, h2⟩ := progress_match_ctors j1' j2' vs'
+    let lem1 : lookup x G = some (.openm x ⟨m, Ks, n, Ts, R⟩) := sorry
+    let ⟨i, b, p, lem2, lem3⟩ := oe lem1 (h2.subst_invariant τ)
+    let lem4 := query_match_implies_pattern_match rfl lem3
+    let σ := Constructor.subst ctors
+    Or.inr ⟨_, .openm_match (σ := σ) h1 lem2 j3 lem4 rfl⟩
   | Or.inr ⟨i, t', r⟩ =>
     let ts' := Fun.Vec.update ts t' i
     let r' : G ⊢ ts i ~> ts' i := by subst ts'; simp; exact r
     Or.inr ⟨_, .openm_congr i r' Fun.Vec.update_neq⟩
 | .mtch (m := m) (S := S) (ss := ss) j1 j2 j3 j4 j5, e =>
-  let j1' := λ i => progress (j1 i) e
+  let j1' := λ i => progress oe (j1 i) e
   match split_all_or_left j1' with
-  | Or.inl vs => sorry
-    -- let j1' : ∀ (i : Fin m), G&Δ,Γ ⊢ ss.to[i] : S.to[i] := j1 |> cast (by simp)
-    -- let j2' : ∀ (i : Fin m), Ty.datatype? G S.to[i] := j2 |> cast (by simp)
-    -- let vs' : ∀ (i : Fin m), Value G ss.to[i] := vs |> cast (by simp)
-    -- let ⟨ctors, h1, h2⟩ := progress_match_ctors j1' j2' vs'
-    -- let ⟨i, h3⟩ := j5 h2
-    -- let lem1 := query_match_implies_pattern_match rfl h3
-    -- let σ := Constructor.subst ctors
-    -- Or.inr ⟨_, .data_match (σ := σ) h1 lem1 rfl⟩
+  | Or.inl vs =>
+    let j1' : ∀ (i : Fin m), G&Δ,Γ ⊢ ss.to[i] : S.to[i] := j1 |> cast (by simp)
+    let j2' : ∀ (i : Fin m), Ty.data? .cls G S.to[i] := j2 |> cast (by simp)
+    let vs' : ∀ (i : Fin m), Value G ss.to[i] := vs |> cast (by simp)
+    let ⟨ctors, h1, h2⟩ := progress_match_ctors j1' j2' vs'
+    let ⟨i, h3⟩ := j5 h2
+    let lem1 := query_match_implies_pattern_match rfl h3
+    let σ := Constructor.subst ctors
+    Or.inr ⟨_, .data_match (σ := σ) h1 lem1 rfl⟩
   | Or.inr ⟨i, t', r⟩ =>
     let ss' := Fun.Vec.update ss t' i
     let r' : G ⊢ ss i ~> ss' i := by subst ss'; simp; exact r
     Or.inr ⟨_, .match_congr i r' Fun.Vec.update_neq⟩
 | .lam j1 j2, e => Or.inl Value.lam
 | .app j1 j2, e =>
-  match progress j1 e with
+  match progress oe j1 e with
   | Or.inl v =>
     match v, j1 with
     | .lam, .lam j3 j4 => Or.inr ⟨_, .beta⟩
@@ -133,7 +156,7 @@ theorem progress :
   | Or.inr ⟨f', r⟩ => Or.inr ⟨_, .app_congr r⟩
 | .lamt j1 j2, e => Or.inl Value.lamt
 | .appt j1 j2 j3, e =>
-  match progress j1 e with
+  match progress oe j1 e with
   | Or.inl v =>
     match v, j1 with
     | .lamt, .lamt j3 j4 => Or.inr ⟨_, .betat⟩
@@ -141,14 +164,14 @@ theorem progress :
   | Or.inr ⟨f', r⟩ => Or.inr ⟨_, .ctor1_congr r⟩
 | .refl j, e => Or.inl Value.refl
 | .cast (R := R) (t := t) j1 j2 j3 e1, e2 =>
-  match progress j2 e2 with
+  match progress oe j2 e2 with
   | Or.inl v =>
     match v, j2 with
     | .refl, .refl j4 => Or.inr ⟨t, .cast⟩
     | .spctor h, j4 => by grind
   | Or.inr ⟨c', r⟩ => Or.inr ⟨.cast R c' t, .cast_congr r⟩
 | .prj j1 j2, e =>
-  match progress j1 e with
+  match progress oe j1 e with
   | Or.inl v =>
     match v, j1, j2 with
     | .refl, .refl j3, .fst_app h => Or.inr ⟨_, .prj_fst_app⟩
@@ -161,18 +184,18 @@ theorem progress :
     | .spctor h, j3, .snd_arrow _ => by grind
   | Or.inr ⟨t', r⟩ => Or.inr ⟨_, .ctor1_congr r⟩
 | .allc j1, e =>
-  match progress j1 (e |> cast (by grind)) with
+  match progress oe j1 (e |> cast (by grind)) with
   | Or.inl v =>
     match v, j1 with
     | .refl, .refl j2 => Or.inr ⟨_, .allc⟩
     | .spctor h, j2 => by grind
   | Or.inr ⟨c', r⟩ => Or.inr ⟨_, .allc_congr r⟩
 | .apptc j1 j2 e1 e2, e3 =>
-  match progress j1 e3, progress j2 e3 with
+  match progress oe j1 e3, progress oe j2 e3 with
   | Or.inl v1, Or.inl v2 =>
     match v1, v2, j1, j2 with
     | .refl, .refl, .refl j3, .refl j4 => Or.inr ⟨_, .apptc⟩
-    | .spctor h, _, j3, j4 => by grind
+    | .spctor h, _, j3, j4
     | _, .spctor h, j3, j4 => by grind
   | Or.inr ⟨f', r⟩, _ => Or.inr ⟨_, .apptc_congr1 r⟩
   | _, Or.inr ⟨a', r⟩ => Or.inr ⟨_, .apptc_congr2 r⟩
